add more sanity checks

Examples/SignedDHKEM/SanityChecks.lean
@@ -18,6 +18,18 @@ theorem liftM_parse_preserves_reachability
   simp only [Traceful.PreservesReachability, Traceful.PreservesReachabilityFrom, liftM, monadLift, MonadLift.monadLift, Traceful.run_mk]
   grind
 
+theorem liftM_kemDecap_preserves_reachability
+  (config: ReachabilityConfig)
+  (sk cipher: Bytes)
+  : (liftM (KEM.kemDecap sk cipher): Traceful Bytes).PreservesReachability config (fun tr => sk.AttackerKnows tr ∧ cipher.AttackerKnows tr) (fun res tr => res.AttackerKnows tr)
+:= by
+  simp only [Traceful.PreservesReachability, Traceful.PreservesReachabilityFrom, liftM, monadLift, MonadLift.monadLift, Traceful.run_mk]
+  intro tr h_reach h_pre
+  apply And.intro
+  · grind
+  have := KEM.kemDecap.attacker_knows sk cipher tr (by grind) (by grind)
+  grind
+
 public
 def honestAttacker: Traceful Unit := do
   let (_, pkHandle, skHandle) ← LongTermKeys.generateKeyPair "SignedDHKEM PKI" "Bob" -- 4
@@ -92,33 +104,39 @@ info: 'DY.Example.SignedDHKEM.honestAttacker_properties' depends on axioms: [pro
 #guard_msgs in
 #print axioms honestAttacker_properties
 
-#exit
 public
-def compromiseClientEphAttacker: Traceful Unit := do
+def breakDhAndKemAttacker: Traceful Unit := do
   honestAttacker
-  let stClientHandle := 6
-  let msgServerHandle := 12
+  let msgClientHandle := 9
+  let msgServerHandle := 15
 
-  let compromiseHandle ← ClientInitiateState.compromise stClientHandle
-  let globalStClientBytes ← Network.receiveMessage compromiseHandle
-  let globalStClient: PersistentLocalState.LocalState ClientInitiateState ← Comparse.parse globalStClientBytes
-  let stClient: ClientInitiateState := globalStClient.state
-
+  let msgClientBytes ← Network.receiveMessage msgClientHandle
+  let msgClient: ClientMessage ← Comparse.parse msgClientBytes
   let msgServerBytes ← Network.receiveMessage msgServerHandle
   let msgServer: ServerMessage ← Comparse.parse msgServerBytes
 
-  let k := Hash.hash (DiffieHellman.dh msgServer.yPk stClient.xSk)
+  let xPkHandle ← Network.sendMessage msgClient.xPk
+  let xSkHandle ← DiffieHellman'.Broken.breakDhPk xPkHandle
+  let xSk ← Network.receiveMessage xSkHandle
+
+  let zPkHandle ← Network.sendMessage msgClient.zPk
+  let zSkHandle ← KEM.Broken.breakKemPk zPkHandle
+  let zSk ← Network.receiveMessage zSkHandle
+
+  let dhss := DiffieHellman'.dh msgServer.yPk xSk
+  let kemss ← KEM.kemDecap zSk msgServer.ct
+  let k := Hash.hash (Concat.concat dhss kemss)
   let _ ← Network.sendMessage k
   return ()
 
-#guard (compromiseClientEphAttacker.run Trace.nil).fst = some ()
+#guard (breakDhAndKemAttacker.run Trace.nil).fst = some ()
 
-theorem compromiseClientEphAttacker_PreservesReachability
-  : compromiseClientEphAttacker.PreservesReachability reachability (fun _ => True) (fun _ _ => True)
+theorem breakDhAndKemAttacker_PreservesReachability
+  : breakDhAndKemAttacker.PreservesReachability reachability (fun _ => True) (fun _ _ => True)
 := by
   unfold Traceful.PreservesReachability
   intro tr h_tr h_pre
-  dsimp only [compromiseClientEphAttacker]
+  dsimp only [breakDhAndKemAttacker]
 
   apply Traceful.PreservesReachabilityFrom_bind
   · apply honestAttacker_PreservesReachability
@@ -127,22 +145,16 @@ theorem compromiseClientEphAttacker_PreservesReachability
   intro _ tr h_post h_tr h_le
 
   apply Traceful.PreservesReachabilityFrom_bind
-  · apply Traceful.PreservesReachability_base (ClientInitiateState.compromise.reachability)
-  · assumption
-  · simp [ClientInitiateState.compromise.reachability]
-  intro compromiseHandle tr h_post h_tr h_le
-
-  apply Traceful.PreservesReachabilityFrom_bind
   · apply Network.receiveMessage.preservesReachability
   · assumption
   · grind
-  intro globalStClientBytes tr h_post h_tr h_le
+  intro msgClientBytes tr h_post h_tr h_le
 
   apply Traceful.PreservesReachabilityFrom_bind
   · apply liftM_parse_preserves_reachability
   · assumption
   · grind
-  intro globalStClient tr h_post h_tr h_le
+  intro msgClient tr h_post h_tr h_le
 
   apply Traceful.PreservesReachabilityFrom_bind
   · apply Network.receiveMessage.preservesReachability
@@ -159,10 +171,56 @@ theorem compromiseClientEphAttacker_PreservesReachability
   apply Traceful.PreservesReachabilityFrom_bind
   · apply Traceful.PreservesReachability_base (Network.reachability)
   · assumption
+  · grind
+  intro xPkHandle tr h_post h_tr h_le
+
+  apply Traceful.PreservesReachabilityFrom_bind
+  · apply Traceful.PreservesReachability_base (DiffieHellman'.Broken.breakDhPk.reachability)
+  · assumption
+  · simp [DiffieHellman'.Broken.breakDhPk.reachability]
+  intro xSkHandle tr h_post h_tr h_le
+
+  apply Traceful.PreservesReachabilityFrom_bind
+  · apply Network.receiveMessage.preservesReachability
+  · assumption
+  · grind
+  intro xSk tr h_post h_tr h_le
+
+  apply Traceful.PreservesReachabilityFrom_bind
+  · apply Traceful.PreservesReachability_base (Network.reachability)
+  · assumption
+  · grind
+  intro zPkHandle tr h_post h_tr h_le
+
+  apply Traceful.PreservesReachabilityFrom_bind
+  · apply Traceful.PreservesReachability_base (KEM.Broken.breakKemPk.reachability)
+  · assumption
+  · simp [KEM.Broken.breakKemPk.reachability]
+  intro zSkHandle tr h_post h_tr h_le
+
+  apply Traceful.PreservesReachabilityFrom_bind
+  · apply Network.receiveMessage.preservesReachability
+  · assumption
+  · grind
+  intro zSk tr h_post h_tr h_le
+
+  apply Traceful.PreservesReachabilityFrom_bind
+  · apply liftM_kemDecap_preserves_reachability
+  · assumption
+  · apply And.intro
+    · grind
+    · grind (gen := 50)
+  intro kemss tr h_post h_tr h_le
+
+  apply Traceful.PreservesReachabilityFrom_bind
+  · apply Traceful.PreservesReachability_base (Network.reachability)
+  · assumption
   · dsimp only
     apply Hash.attacker_knows_hash
-    apply DiffieHellman.attacker_knows_dh
-    · grind
+    apply Concat.attacker_knows_concat
+    · apply DiffieHellman'.attacker_knows_dh
+      · grind (gen := 50)
+      · grind
     · grind
   intro _ tr h_post h_tr h_le
 
@@ -171,20 +229,20 @@ theorem compromiseClientEphAttacker_PreservesReachability
   grind
 
 public
-theorem compromiseClientEphAttacker_properties:
-  let tr := (compromiseClientEphAttacker.run (Trace.nil)).snd.val
+theorem breakDhAndKemAttacker_properties:
+  let tr := (breakDhAndKemAttacker.run (Trace.nil)).snd.val
   tr.Reachable reachability ∧
-  ∃ t1 xPk yPk k,
-    tr.EventLoggedAt (SignedDHEvent.ClientFinishEvent "Alice" "Bob" xPk yPk k) t1 ∧
+  ∃ t1 xPk yPk zPk k,
+    tr.EventLoggedAt (SignedDHKEMEvent.ClientFinishEvent "Alice" "Bob" xPk yPk zPk k) t1 ∧
     k.AttackerKnows tr
 := by
   intro tr
   refine ⟨ ?_, ?_ ⟩
-  · apply Traceful.PreservesReachability_to_Reachable compromiseClientEphAttacker_PreservesReachability
+  · apply Traceful.PreservesReachability_to_Reachable breakDhAndKemAttacker_PreservesReachability
     grind
   suffices
-      ∃ t1 t2 xPk yPk k,
-        tr.EventLoggedAt (SignedDHEvent.ClientFinishEvent "Alice" "Bob" xPk yPk k) t1 ∧
+      ∃ t1 t2 xPk yPk zPk k,
+        tr.EventLoggedAt (SignedDHKEMEvent.ClientFinishEvent "Alice" "Bob" xPk yPk zPk k) t1 ∧
         tr.MessageSentAt k t2
   by
     have := Trace.MessageSentAt_implies_AttackerKnows
@@ -192,84 +250,81 @@ theorem compromiseClientEphAttacker_properties:
   simp only [DY.Trace.EventLoggedAt_eq_getEventAt]
   simp only [DY.Trace.MessageSentAt_eq_getMessageSentAt]
   let witness :=
-    match (Trace.getEventAt SignedDHEvent 13 tr) with
-    | some (SignedDHEvent.ClientFinishEvent _ _ xPk yPk k) => (xPk, yPk, k)
-    | _ => (Comparse.BytesLike.empty, Comparse.BytesLike.empty, Comparse.BytesLike.empty)
-  refine ⟨ 13, 17, witness.fst, witness.snd.fst, witness.snd.snd, ?_ ⟩
+    match (Trace.getEventAt SignedDHKEMEvent 16 tr) with
+    | some (SignedDHKEMEvent.ClientFinishEvent _ _ xPk yPk zPk k) => (xPk, yPk, zPk, k)
+    | _ => (Comparse.BytesLike.empty, Comparse.BytesLike.empty, Comparse.BytesLike.empty, Comparse.BytesLike.empty)
+  refine ⟨ 16, 24, witness.fst, witness.snd.fst, witness.snd.snd.fst, witness.snd.snd.snd, ?_ ⟩
   native_decide
 
 /--
-info: 'DY.Example.SignedDH.compromiseClientEphAttacker_properties' depends on axioms: [propext,
+info: 'DY.Example.SignedDHKEM.breakDhAndKemAttacker_properties' depends on axioms: [propext,
  Classical.choice,
  Quot.sound,
- compromiseClientEphAttacker_properties._native.native_decide.ax_1_7]
+ breakDhAndKemAttacker_properties._native.native_decide.ax_1_7]
 -/
 #guard_msgs in
-#print axioms compromiseClientEphAttacker_properties
+#print axioms breakDhAndKemAttacker_properties
+
 
 public
-def compromiseSigKeyAttacker: Traceful Unit := do
-  let (_, pkHandle, skHandle) ← LongTermKeys.generateKeyPair "SignedDH PKI" "Bob" -- 4
-  let compromiseHandle ← LongTermKeys.compromisePrivateKey "SignedDH PKI" skHandle -- 2
-  let globalStSigkeyBytes ← Network.receiveMessage compromiseHandle
-  let globalStSigkey: PersistentLocalState.LocalState (LongTermKeys.SecretKeyState "SignedDH PKI") ← Comparse.parse globalStSigkeyBytes
-  let sigKey := globalStSigkey.state.sk
+def breakSigKeyAttacker: Traceful Unit := do
+  let (serverVkHandle, pkHandle, _skHandle) ← LongTermKeys.generateKeyPair "SignedDHKEM PKI" "Bob" -- 4
+  let serverSkHandle ← Signature'.Broken.breakVk serverVkHandle -- 2
+  let sigKey ← Network.receiveMessage serverSkHandle
 
-  let (stClientHandle, msgClientHandle) ← Client.initiate "Alice" -- 4
+  let (dhStClientHandle, kemStClientHandle, msgClientHandle) ← Client.initiate "Alice" -- 6
 
   let msgClientBytes ← Network.receiveMessage msgClientHandle
   let msgClient: ClientMessage ← Comparse.parse msgClientBytes
   let xPk := msgClient.xPk
+  let zPk := msgClient.zPk
 
   let ySk := Literal.literalToBytes "00000000000000000000000000000000".toByteArray
-  let yPk := DiffieHellman.dh_pk ySk
-  let k := Hash.hash (DiffieHellman.dh xPk ySk)
+  let yPk := DiffieHellman'.dh_pk ySk
+  let dhss := DiffieHellman'.dh xPk ySk
+  let entropy := Literal.literalToBytes "00000000000000000000000000000000".toByteArray
+  let (ct, kemss) := KEM.kemEncap zPk entropy
+  let k := Hash.hash (Concat.concat dhss kemss)
+
   let sigNonce := Literal.literalToBytes "00000000000000000000000000000000".toByteArray
-  let sig := Signature.sign sigKey sigNonce (Comparse.serialize ({xPk, yPk}: SigInput))
-  let msgServerHandle ← Network.sendMessage (Comparse.serialize ({ yPk, sig } : ServerMessage)) -- 1
-  let _ ← Client.finish "Alice" "Bob" pkHandle msgServerHandle stClientHandle -- 2
+  let sig := Signature'.sign sigKey sigNonce (Comparse.serialize ({xPk, yPk, zPk, ct}: SigInput))
+  let msgServerHandle ← Network.sendMessage (Comparse.serialize ({ yPk, ct, sig } : ServerMessage)) -- 1
+  let _ ← Client.finish "Alice" "Bob" pkHandle msgServerHandle dhStClientHandle kemStClientHandle -- 2
   let _ ← Network.sendMessage k -- 1
   return ()
 
-#guard (compromiseSigKeyAttacker.run Trace.nil).fst = some ()
+#guard (breakSigKeyAttacker.run Trace.nil).fst = some ()
 
-theorem compromiseSigKeyAttacker_PreservesReachability
-  : compromiseSigKeyAttacker.PreservesReachability reachability (fun _ => True) (fun _ _ => True)
+theorem breakSigKeyAttacker_PreservesReachability
+  : breakSigKeyAttacker.PreservesReachability reachability (fun _ => True) (fun _ _ => True)
 := by
   unfold Traceful.PreservesReachability
   intro tr h_tr h_pre
-  dsimp only [compromiseSigKeyAttacker]
+  dsimp only [breakSigKeyAttacker]
 
   apply Traceful.PreservesReachabilityFrom_bind
-  · apply Traceful.PreservesReachability_base (LongTermKeys.generateKeyPair.reachability "SignedDH PKI")
+  · apply Traceful.PreservesReachability_base (LongTermKeys.generateKeyPair.reachability "SignedDHKEM PKI")
   · assumption
   · simp [LongTermKeys.generateKeyPair.reachability]
   intro ⟨ _, pkHandle, skHandle ⟩ tr h_post h_tr h_le
 
   apply Traceful.PreservesReachabilityFrom_bind
-  · apply Traceful.PreservesReachability_base (LongTermKeys.compromisePrivateKey.reachability "SignedDH PKI")
+  · apply Traceful.PreservesReachability_base (Signature'.Broken.breakVk.reachability)
   · assumption
-  · simp [LongTermKeys.compromisePrivateKey.reachability]
-  intro compromiseHandle tr h_post h_tr h_le
+  · simp [Signature'.Broken.breakVk.reachability]
+  intro serverSkHandle tr h_post h_tr h_le
 
   apply Traceful.PreservesReachabilityFrom_bind
   · apply Network.receiveMessage.preservesReachability
   · assumption
   · grind
-  intro globalStSigkeyBytes tr h_post h_tr h_le
+  intro sigKey tr h_post h_tr h_le
 
-  apply Traceful.PreservesReachabilityFrom_bind
-  · apply liftM_parse_preserves_reachability
-  · assumption
-  · grind
-  intro globalStSigkey tr h_post h_tr h_le
-
-  dsimp
   apply Traceful.PreservesReachabilityFrom_bind
   · apply Traceful.PreservesReachability_base (Client.initiate.reachability)
   · assumption
   · simp [Client.initiate.reachability]
-  intro ⟨ stClientHandle, msgClientHandle ⟩ tr h_post h_tr h_le
+  intro ⟨ dhStClientHandle, kemStClientHandle, msgClientHandle ⟩ tr h_post h_tr h_le
 
   apply Traceful.PreservesReachabilityFrom_bind
   · apply Network.receiveMessage.preservesReachability
@@ -288,20 +343,30 @@ theorem compromiseSigKeyAttacker_PreservesReachability
   · assumption
   · simp only [Comparse.AttackerKnows_serialize, ServerMessage.IsWellFormed_eq]
     apply And.intro
-    · apply DiffieHellman.attacker_knows_dh_pk
+    · apply DiffieHellman'.attacker_knows_dh_pk
       apply Literal.attacker_knows_literalToBytes
-    apply Signature.attacker_knows_sign
-    · grind (ematch := 10)
+    apply And.intro
+    · have := KEM.kemEncap.attacker_knows
+      have := Literal.attacker_knows_literalToBytes
+      grind
+    apply Signature'.attacker_knows_sign
+    · grind
     · apply Literal.attacker_knows_literalToBytes
     · simp only [Comparse.AttackerKnows_serialize, SigInput.IsWellFormed_eq]
       apply And.intro
       · grind
-      · apply DiffieHellman.attacker_knows_dh_pk
+      apply And.intro
+      · apply DiffieHellman'.attacker_knows_dh_pk
         apply Literal.attacker_knows_literalToBytes
+      apply And.intro
+      · grind
+      have := KEM.kemEncap.attacker_knows
+      have := Literal.attacker_knows_literalToBytes
+      grind
   intro msgServerHandle tr h_post h_tr h_le
 
   apply Traceful.PreservesReachabilityFrom_bind
-  · apply Traceful.PreservesReachability_base (Client.finish.reachability) _ ("Alice", "Bob", pkHandle, msgServerHandle, stClientHandle)
+  · apply Traceful.PreservesReachability_base (Client.finish.reachability) _ ("Alice", "Bob", pkHandle, msgServerHandle, dhStClientHandle, kemStClientHandle)
   · assumption
   · simp [Client.finish.reachability]
   intro _ tr h_post h_tr h_le
@@ -311,9 +376,14 @@ theorem compromiseSigKeyAttacker_PreservesReachability
   · assumption
   · dsimp only
     apply Hash.attacker_knows_hash
-    apply DiffieHellman.attacker_knows_dh
-    · grind
-    · apply Literal.attacker_knows_literalToBytes
+    apply Concat.attacker_knows_concat
+    · apply DiffieHellman'.attacker_knows_dh
+      · grind
+      · apply Literal.attacker_knows_literalToBytes
+    · have: msgClient.zPk.AttackerKnows tr := by grind
+      have := KEM.kemEncap.attacker_knows
+      have := Literal.attacker_knows_literalToBytes
+      grind
   intro _ tr h_post h_tr h_le
 
   apply Traceful.PreservesReachabilityFrom_pure
@@ -321,20 +391,20 @@ theorem compromiseSigKeyAttacker_PreservesReachability
   grind
 
 public
-theorem compromiseSigKeyAttacker_properties:
-  let tr := (compromiseSigKeyAttacker.run (Trace.nil)).snd.val
+theorem breakSigKeyAttacker_properties:
+  let tr := (breakSigKeyAttacker.run (Trace.nil)).snd.val
   tr.Reachable reachability ∧
-  ∃ t1 xPk yPk k,
-    tr.EventLoggedAt (SignedDHEvent.ClientFinishEvent "Alice" "Bob" xPk yPk k) t1 ∧
+  ∃ t1 xPk yPk zPk k,
+    tr.EventLoggedAt (SignedDHKEMEvent.ClientFinishEvent "Alice" "Bob" xPk yPk zPk k) t1 ∧
     k.AttackerKnows tr
 := by
   intro tr
   refine ⟨ ?_, ?_ ⟩
-  · apply Traceful.PreservesReachability_to_Reachable compromiseSigKeyAttacker_PreservesReachability
+  · apply Traceful.PreservesReachability_to_Reachable breakSigKeyAttacker_PreservesReachability
     grind
   suffices
-    ∃ t1 t2 xPk yPk k,
-      tr.EventLoggedAt (SignedDHEvent.ClientFinishEvent "Alice" "Bob" xPk yPk k) t1 ∧
+    ∃ t1 t2 xPk yPk zPk k,
+      tr.EventLoggedAt (SignedDHKEMEvent.ClientFinishEvent "Alice" "Bob" xPk yPk zPk k) t1 ∧
       tr.MessageSentAt k t2
   by
     have := Trace.MessageSentAt_implies_AttackerKnows
@@ -342,19 +412,19 @@ theorem compromiseSigKeyAttacker_properties:
   simp only [DY.Trace.EventLoggedAt_eq_getEventAt]
   simp only [DY.Trace.MessageSentAt_eq_getMessageSentAt]
   let witness :=
-    match (Trace.getEventAt SignedDHEvent 11 tr) with
-    | some (SignedDHEvent.ClientFinishEvent _ _ xPk yPk k) => (xPk, yPk, k)
-    | _ => (Comparse.BytesLike.empty, Comparse.BytesLike.empty, Comparse.BytesLike.empty)
-  refine ⟨ 11, 13, witness.fst, witness.snd.fst, witness.snd.snd, ?_ ⟩
+    match (Trace.getEventAt SignedDHKEMEvent 13 tr) with
+    | some (SignedDHKEMEvent.ClientFinishEvent _ _ xPk yPk zPk k) => (xPk, yPk, zPk, k)
+    | _ => (Comparse.BytesLike.empty, Comparse.BytesLike.empty, Comparse.BytesLike.empty, Comparse.BytesLike.empty)
+  refine ⟨ 13, 15, witness.fst, witness.snd.fst, witness.snd.snd.fst, witness.snd.snd.snd, ?_ ⟩
   native_decide
 
 /--
-info: 'DY.Example.SignedDH.compromiseSigKeyAttacker_properties' depends on axioms: [propext,
+info: 'DY.Example.SignedDHKEM.breakSigKeyAttacker_properties' depends on axioms: [propext,
  Classical.choice,
  Quot.sound,
- compromiseSigKeyAttacker_properties._native.native_decide.ax_1_7]
+ breakSigKeyAttacker_properties._native.native_decide.ax_1_7]
 -/
 #guard_msgs in
-#print axioms compromiseSigKeyAttacker_properties
+#print axioms breakSigKeyAttacker_properties
 
 end DY.Example.SignedDHKEM
